Allocate.v
@@ -26,8 +26,8 @@ Include MSSMorph M.
 
     jww (2014-10-01): Prove that it always succeeds. *)
 
-Definition splitCurrentInterval {pre} (before : option nat)
-  : SState pre SSMorphHasLen SSMorphStHasLen unit.
+Definition splitCurrentInterval {pre P} `{HasWork P} (before : option nat)
+  : SState pre P SSMorphStHasLen unit.
   (* jww (2014-09-26): NYI *)
 Admitted.
 
@@ -44,62 +44,60 @@ Admitted.
 (** If [tryAllocateFreeReg] fails to allocate a register, the [ScanState] is
     left unchanged.  If it succeeds, or is forced to split [current], then a
     register will have been assigned. *)
-Definition tryAllocateFreeReg {pre}
-  : SState pre SSMorphHasLen SSMorphHasLen
-           (option (SState pre SSMorphHasLen SSMorphSt PhysReg)) :=
-  withLenCursor $ fun sd cur =>
-  let current := curInterval cur in
-  let sd := curStateDesc cur in
+Definition tryAllocateFreeReg {pre P} `{W : HasWork P}
+  : SState pre P P (option (SState pre P SSMorphSt PhysReg)) :=
+  withCursor $ fun sd cur =>
+    let current := curInterval cur in
+    let sd := curStateDesc cur in
 
-  (* set freeUntilPos of all physical registers to maxInt
-     for each interval it in active do
-       freeUntilPos[it.reg] = 0
-     for each interval it in inactive intersecting with current do
-       freeUntilPos[it.reg] = next intersection of it with current *)
-  let go n := fold_left (fun v i => atIntervalReg i v (n i)) in
-  let freeUntilPos' := go (fun _ => Some 0)
-                          (active sd) (V.const None maxReg) in
-  let intersectingIntervals :=
-      filter (fun x => anyRangeIntersects current (getInterval x))
-             (inactive sd) in
-  let freeUntilPos :=
-      go (fun i => firstIntersectionPoint (getInterval i) current)
-         intersectingIntervals freeUntilPos' in
+    (* set freeUntilPos of all physical registers to maxInt
+       for each interval it in active do
+         freeUntilPos[it.reg] = 0
+       for each interval it in inactive intersecting with current do
+         freeUntilPos[it.reg] = next intersection of it with current *)
+    let go n := fold_left (fun v i => atIntervalReg i v (n i)) in
+    let freeUntilPos' := go (fun _ => Some 0)
+                            (active sd) (V.const None maxReg) in
+    let intersectingIntervals :=
+        filter (fun x => anyRangeIntersects current (getInterval x))
+               (inactive sd) in
+    let freeUntilPos :=
+        go (fun i => firstIntersectionPoint (getInterval i) current)
+           intersectingIntervals freeUntilPos' in
 
-  (* reg = register with highest freeUntilPos *)
-  (* mres = highest use position of the found register *)
-  let (reg, mres) := registerWithHighestPos freeUntilPos in
+    (* reg = register with highest freeUntilPos *)
+    (* mres = highest use position of the found register *)
+    let (reg, mres) := registerWithHighestPos freeUntilPos in
 
-  (** [moveUnhandledToActive] not only moves an [IntervalId] from the
-      [unhandled] list to the [active] list in the current [ScanStateDesc], it
-      also assignments a register to that newly active interval, which can be
-      accessed by calling [getAssignment]. *)
+    (** [moveUnhandledToActive] not only moves an [IntervalId] from the
+        [unhandled] list to the [active] list in the current [ScanStateDesc], it
+        also assignments a register to that newly active interval, which can be
+        accessed by calling [getAssignment]. *)
 
-  let success := moveUnhandledToActive reg ;;; return_ reg in
-  let maction :=
-      match mres with
-      | None => Some success
-      | Some n =>
-        (* if freeUntilPos[reg] = 0 then
-             // no register available without spilling
-             allocation failed
-           else if current ends before freeUntilPos[reg] then
-             // register available for the whole interval
-             current.reg = reg
-           else
-             // register available for the first part of the interval
-             current.reg = reg
-             split current before freeUntilPos[reg] *)
-        if beq_nat n 0
-        then None
-        else Some (if intervalEnd current <? n
-                   then success
-                   else splitCurrentInterval (Some n) ;;;
-                        weakenStHasLenToHasLen ;;;
-                        moveUnhandledToActive reg ;;;
-                        return_ reg)
-      end in
-  return_ maction.
+    let success := moveUnhandledToActive reg ;;; return_ reg in
+    let maction :=
+        match mres with
+        | None => Some success
+        | Some n =>
+          (* if freeUntilPos[reg] = 0 then
+               // no register available without spilling
+               allocation failed
+             else if current ends before freeUntilPos[reg] then
+               // register available for the whole interval
+               current.reg = reg
+             else
+               // register available for the first part of the interval
+               current.reg = reg
+               split current before freeUntilPos[reg] *)
+          if beq_nat n 0
+          then None
+          else Some (if intervalEnd current <? n
+                     then success
+                     else splitCurrentInterval (Some n) ;;;
+                          moveUnhandledToActive reg ;;;
+                          return_ reg)
+        end in
+    return_ maction.
 
 Definition nextUseAfter `(curId : Interval desc) (pos : nat) : option nat.
   (* jww (2014-09-26): NYI *)
@@ -109,12 +107,12 @@ Definition firstUseReqReg `(curId : Interval desc) : option nat.
   (* jww (2014-10-01): NYI *)
 Admitted.
 
-Definition assignSpillSlotToCurrent {pre}
-  : SState pre SSMorphHasLen SSMorphHasLen unit.
+Definition assignSpillSlotToCurrent {pre P} `{HasWork P}
+  : SState pre P P unit.
   (* jww (2014-09-26): NYI *)
 Admitted.
 
-Definition intersectsWithFixedInterval {pre P} (reg : PhysReg)
+Definition intersectsWithFixedInterval {pre P} `{HasWork P} (reg : PhysReg)
   (* jww (2014-10-02): This needs to say "it has to have Len in it" *)
   : SState pre P P (option nat).
   (* jww (2014-10-01): NYI *)
@@ -123,75 +121,73 @@ Admitted.
 (** If [allocateBlockedReg] fails, it's possible no register was assigned and
     that the only outcome was to split one or more intervals.  In either case,
     the change to the [ScanState] must be a productive one. *)
-Definition allocateBlockedReg {pre}
-  : SState pre SSMorphHasLen SSMorphSt (option PhysReg) :=
-  withLenCursor $ fun sd cur =>
-  let st      := curState cur in
-  let current := curInterval cur in
-  let start   := intervalStart current in
-  let pos     := curPosition cur in
+Definition allocateBlockedReg {pre P} `{HasWork P}
+  : SState pre P SSMorphSt (option PhysReg) :=
+  withCursor $ fun sd cur =>
+    let st      := curState cur in
+    let current := curInterval cur in
+    let start   := intervalStart current in
+    let pos     := curPosition cur in
 
-  (* set nextUsePos of all physical registers to maxInt
-     for each interval it in active do
-       nextUsePos[it.reg] = next use of it after start of current
-     for each interval it in inactive intersecting with current do
-       nextUsePos[it.reg] = next use of it after start of current *)
-  let go := fold_left (fun v i =>
-              atIntervalReg i v (nextUseAfter (getInterval i) start)) in
-  let nextUsePos' := go (active sd) (V.const None maxReg) in
-  let intersectingIntervals :=
-      filter (fun x => anyRangeIntersects current (getInterval x))
-             (inactive sd) in
-  let nextUsePos := go intersectingIntervals nextUsePos' in
+    (* set nextUsePos of all physical registers to maxInt
+       for each interval it in active do
+         nextUsePos[it.reg] = next use of it after start of current
+       for each interval it in inactive intersecting with current do
+         nextUsePos[it.reg] = next use of it after start of current *)
+    let go := fold_left (fun v i =>
+                atIntervalReg i v (nextUseAfter (getInterval i) start)) in
+    let nextUsePos' := go (active sd) (V.const None maxReg) in
+    let intersectingIntervals :=
+        filter (fun x => anyRangeIntersects current (getInterval x))
+               (inactive sd) in
+    let nextUsePos := go intersectingIntervals nextUsePos' in
 
-  (* reg = register with highest nextUsePos *)
-  (* mres = highest use position of the found register *)
-  let (reg, mres) := registerWithHighestPos nextUsePos in
+    (* reg = register with highest nextUsePos *)
+    (* mres = highest use position of the found register *)
+    let (reg, mres) := registerWithHighestPos nextUsePos in
 
-  (* if first usage of current is after nextUsePos[reg] then
-       // all other intervals are used before current, so it is best
-       // to spill current itself
-       assign spill slot to current
-       split current before its first use position that requires a register
-     else
-       // spill intervals that currently block reg
-       current.reg = reg
-       split active interval for reg at position
-       split any inactive interval for reg at the end of its lifetime hole *)
+    (* if first usage of current is after nextUsePos[reg] then
+         // all other intervals are used before current, so it is best
+         // to spill current itself
+         assign spill slot to current
+         split current before its first use position that requires a register
+       else
+         // spill intervals that currently block reg
+         current.reg = reg
+         split active interval for reg at position
+         split any inactive interval for reg at the end of its lifetime hole *)
 
-  (* // make sure that current does not intersect with
-     // the fixed interval for reg
-     if current intersects with the fixed interval for reg then
-       split current before this intersection *)
-  if (match mres with
-      | None   => false
-      | Some n => n <? start
-      end)
-  then
-    assignSpillSlotToCurrent ;;;
-    splitCurrentInterval (firstUseReqReg current) ;;;
+    (* // make sure that current does not intersect with
+       // the fixed interval for reg
+       if current intersects with the fixed interval for reg then
+         split current before this intersection *)
+    if (match mres with
+        | None   => false
+        | Some n => n <? start
+        end)
+    then
+      assignSpillSlotToCurrent ;;;
+      splitCurrentInterval (firstUseReqReg current) ;;;
 
-    mloc <<- intersectsWithFixedInterval reg ;
-    match mloc with
-    | Some n => weakenStHasLenToHasLen ;;;
-                splitCurrentInterval (Some n)
-    | None   => return_ tt
-    end ;;;
-    weakenStHasLenToSt ;;;
-    return_ None
-  else
-    splitActiveIntervalForReg reg pos ;;;
-    splitAnyInactiveIntervalForReg reg ;;;
+      mloc <<- intersectsWithFixedInterval reg ;
+      match mloc with
+      | Some n => splitCurrentInterval (Some n)
+      | None   => return_ tt
+      end ;;;
+      weakenStHasLenToSt ;;;
+      return_ None
+    else
+      splitActiveIntervalForReg reg pos ;;;
+      splitAnyInactiveIntervalForReg reg ;;;
 
-    mloc <<- intersectsWithFixedInterval reg ;
-    match mloc with
-    | Some n => splitCurrentInterval (Some n) ;;;
-                weakenStHasLenToHasLen
-    | None   => return_ tt
-    end ;;;
-
-    moveUnhandledToActive reg ;;;
-    return_ (Some reg).
+      mloc <<- intersectsWithFixedInterval reg ;
+      match mloc
+      with
+      | Some n => splitCurrentInterval (Some n) ;;;
+                  moveUnhandledToActive reg
+      | None   => moveUnhandledToActive reg
+      end ;;;
+      return_ (Some reg).
 
 Definition checkActiveIntervals {pre} (pos : nat)
   : SState pre SSMorphLen SSMorphLen unit :=
@@ -252,26 +248,25 @@ Definition checkInactiveIntervals {pre} (pos : nat)
 Definition handleInterval {pre}
   : SState pre SSMorphHasLen SSMorphSt (option PhysReg) :=
   (* position = start position of current *)
-  withLenCursor $ fun _ cur =>
-  let position := curPosition cur in
+  withCursor $ fun _ cur =>
+    let position := curPosition cur in
 
-  (* // check for intervals in active that are handled or inactive *)
-  liftLen (checkActiveIntervals position) ;;;
-  (* // check for intervals in inactive that are handled or active *)
-  liftLen (checkInactiveIntervals position) ;;;
+    (* // check for intervals in active that are handled or inactive *)
+    liftLen (checkActiveIntervals position) ;;;
+    (* // check for intervals in inactive that are handled or active *)
+    liftLen (checkInactiveIntervals position) ;;;
 
-  (* // find a register for current
-     tryAllocateFreeReg
-     if allocation failed then
-       allocateBlockedReg
-     if current has a register assigned then
-       add current to active (done by the helper functions) *)
-  mres <<- tryAllocateFreeReg ;
-  match mres with
-  | Some x => reg <<- x ;
-              return_ (Some reg)
-  | None   => allocateBlockedReg
-  end.
+    (* // find a register for current
+       tryAllocateFreeReg
+       if allocation failed then
+         allocateBlockedReg
+       if current has a register assigned then
+         add current to active (done by the helper functions) *)
+    mres <<- tryAllocateFreeReg ;
+    match mres with
+    | Some x => imap (@Some _) x
+    | None   => allocateBlockedReg
+    end.
 
 Function linearScan (sd : ScanStateDesc) (st : ScanState sd)
   {measure unhandledExtent sd} : { sd' : ScanStateDesc | ScanState sd' } :=
